WIP on byte-aligned DNS decoder.

src/BinEncoders/Env/Examples/SimpleDnsOpt.v
@@ -13,7 +13,7 @@ Require Import
         Fiat.QueryStructure.Specification.Representation.Notations
         Fiat.QueryStructure.Specification.Representation.Heading
         Fiat.QueryStructure.Specification.Representation.Tuple
-        Fiat.BinEncoders.Env.BinLib.Core
+        Fiat.BinEncoders.Env.BinLib.AlignedByteString
         Fiat.BinEncoders.Env.BinLib.AlignWord
         Fiat.BinEncoders.Env.Common.Specs
         Fiat.BinEncoders.Env.Common.Compose
@@ -1002,6 +1002,37 @@ Section DnsPacket.
       intros; apply FixList_decode_correct with (A_predicate := resourceRecord_OK)
     end.
 
+  Lemma addD_addD_plus :
+    forall (cd : CacheDecode) (n m : nat), addD (addD cd n) m = addD cd (n + m).
+    simpl; intros.
+    destruct (fst cd); simpl; eauto.
+    repeat (find_if_inside; simpl); eauto.
+    f_equal; f_equal.
+    rewrite !natToWord_plus.
+    rewrite !natToWord_wordToNat.
+    rewrite wplus_assoc; reflexivity.
+    rewrite !natToWord_plus in l0.
+    rewrite !natToWord_wordToNat in l0.
+    elimtype False.
+    apply n0.
+    rewrite <- (natToWord_wordToNat w) in l0.
+    rewrite <- natToWord_plus in l0.
+    rewrite wordToNat_natToWord_idempotent in l0.
+    omega.
+    apply Nomega.Nlt_in; rewrite Nnat.Nat2N.id, Npow2_nat; assumption.
+    elimtype False.
+    apply n0.
+    rewrite <- (natToWord_wordToNat w).
+    rewrite !natToWord_plus.
+    rewrite !wordToNat_natToWord_idempotent.
+    rewrite <- natToWord_plus.
+    rewrite !wordToNat_natToWord_idempotent.
+    omega.
+    apply Nomega.Nlt_in; rewrite Nnat.Nat2N.id, Npow2_nat; assumption.
+    apply Nomega.Nlt_in; rewrite Nnat.Nat2N.id, Npow2_nat; omega.
+    omega.
+  Qed.
+
 Ltac synthesize_decoder_ext
      transformer
      decode_step'
@@ -1013,6 +1044,17 @@ Ltac synthesize_decoder_ext
     repeat first [decode_step' idtac | decode_step determineHooks]
   | cbv beta; synthesize_cache_invariant' idtac
   |  ].
+
+Definition ByteAlignedCorrectDecoderFor {A} {cache : Cache}
+           Invariant FormatSpec :=
+  { decodePlusCacheInv |
+      exists P_inv,
+        (cache_inv_Property (snd decodePlusCacheInv) P_inv
+         -> encode_decode_correct_f (A := A) cache transformer Invariant (fun _ _ => True)
+                                    FormatSpec
+                                    (fst decodePlusCacheInv)
+                                    (snd decodePlusCacheInv))
+        /\ cache_inv_Property (snd decodePlusCacheInv) P_inv}.
 
   Definition packet_decoder
     : CorrectDecoderFor DNS_Packet_OK encode_packet_Spec.
@@ -1050,40 +1092,23 @@ Ltac synthesize_decoder_ext
     first [ apply DecodeBindOpt2_under_bind; simpl; intros
             | eapply optimize_under_if_bool; simpl; intros
             | eapply optimize_under_if; simpl; intros].
-
-  Lemma If_Opt_Then_Else_DecodeBindOpt_swap {A B C ResultT : Type}
-    : forall (a_opt : option A)
-             (b : B)
-             (cd : CacheDecode)
-             (dec_c : B -> CacheDecode -> option (C * B * CacheDecode))
-             (k : A -> C -> B -> CacheDecode -> option (ResultT * B * CacheDecode)),
-             (`(a, b', cd') <- Ifopt a_opt as a Then Some (a, b, cd) Else None;
-              `(c, b', cd') <- dec_c b' cd';
-              k a c b' cd') =
-             (`(c, b', cd') <- dec_c b cd;
-              `(a, b', cd') <- Ifopt a_opt as a Then Some (a, b', cd') Else None;
-              k a c b' cd').
-  Proof.
-    destruct a_opt; simpl; intros; eauto.
-    destruct (dec_c b cd) as [ [ [? ?] [ ? ? ] ] | ]; reflexivity.
-  Qed.
-  rewrite If_Opt_Then_Else_DecodeBindOpt_swap.
+    rewrite (If_Opt_Then_Else_DecodeBindOpt_swap (cache := dns_list_cache)).
+    first [ apply DecodeBindOpt2_under_bind; simpl; intros
+          | eapply optimize_under_if_bool; simpl; intros
+          | eapply optimize_under_if; simpl; intros].
+    rewrite (If_Opt_Then_Else_DecodeBindOpt_swap (cache := dns_list_cache)).
+    first [ apply DecodeBindOpt2_under_bind; simpl; intros
+          | eapply optimize_under_if_bool; simpl; intros
+          | eapply optimize_under_if; simpl; intros].
+    rewrite (If_Opt_Then_Else_DecodeBindOpt_swap (cache := dns_list_cache)).
+    first [ apply DecodeBindOpt2_under_bind; simpl; intros
+            | eapply optimize_under_if_bool; simpl; intros
+            | eapply optimize_under_if; simpl; intros].
+    rewrite (If_Opt_Then_Else_DecodeBindOpt_swap (cache := dns_list_cache)).
   first [ apply DecodeBindOpt2_under_bind; simpl; intros
             | eapply optimize_under_if_bool; simpl; intros
             | eapply optimize_under_if; simpl; intros].
-  rewrite If_Opt_Then_Else_DecodeBindOpt_swap.
-  first [ apply DecodeBindOpt2_under_bind; simpl; intros
-            | eapply optimize_under_if_bool; simpl; intros
-            | eapply optimize_under_if; simpl; intros].
-  rewrite If_Opt_Then_Else_DecodeBindOpt_swap.
-  first [ apply DecodeBindOpt2_under_bind; simpl; intros
-            | eapply optimize_under_if_bool; simpl; intros
-            | eapply optimize_under_if; simpl; intros].
-  rewrite If_Opt_Then_Else_DecodeBindOpt_swap.
-  first [ apply DecodeBindOpt2_under_bind; simpl; intros
-            | eapply optimize_under_if_bool; simpl; intros
-            | eapply optimize_under_if; simpl; intros].
-  rewrite If_Opt_Then_Else_DecodeBindOpt_swap.
+  rewrite (If_Opt_Then_Else_DecodeBindOpt_swap (cache := dns_list_cache)).
   first [ apply DecodeBindOpt2_under_bind; simpl; intros
             | eapply optimize_under_if_bool; simpl; intros
             | eapply optimize_under_if; simpl; intros].
@@ -1091,26 +1116,7 @@ Ltac synthesize_decoder_ext
   first [ apply DecodeBindOpt2_under_bind; simpl; intros
             | eapply optimize_under_if_bool; simpl; intros
             | eapply optimize_under_if; simpl; intros].
-  Lemma If_Then_Else_Bind {sz}  {B C ResultT : Type}
-  : forall (w w' : word sz)
-           (b : B)
-           (cd : CacheDecode)
-           (dec_c : B -> CacheDecode -> option (C * B * CacheDecode))
-           (k : C -> B -> CacheDecode -> option (ResultT * B * CacheDecode)),
-             (if weq w w' then
-                `(c, b', cd') <- dec_c b cd;
-                  k c b' cd'
-              else
-                None) =
-             (`(c, b', cd') <- dec_c b cd;
-                if weq w w' then
-                  k c b' cd'
-                else None).
-  Proof.
-    intros; find_if_inside; eauto.
-    destruct (dec_c b cd) as [ [ [? ?] [ ? ? ] ] | ]; reflexivity.
-  Qed.
-  rewrite If_Then_Else_Bind.
+  rewrite (If_Then_Else_Bind (cache := dns_list_cache)).
   unfold decode_enum at 1.
   repeat (try rewrite !DecodeBindOpt2_assoc;
           try rewrite !Bool.andb_true_r;
@@ -1119,64 +1125,598 @@ Ltac synthesize_decoder_ext
           try rewrite !optimize_if_bind2_bool).
   higher_order_reflexivity.
   set_refine_evar.
-  Lemma  addD_addD_plus :
-    forall (cd : CacheDecode) (n m : nat), addD (addD cd n) m = addD cd (n + m).
-    simpl; intros.
-    destruct (fst cd); simpl; eauto.
-    repeat (find_if_inside; simpl); eauto.
-    f_equal; f_equal.
-    rewrite !natToWord_plus.
-    rewrite !natToWord_wordToNat.
-    rewrite wplus_assoc; reflexivity.
-    rewrite !natToWord_plus in l0.
-    rewrite !natToWord_wordToNat in l0.
-    elimtype False.
-    apply n0.
-    rewrite <- (natToWord_wordToNat w) in l0.
-    rewrite <- natToWord_plus in l0.
-    rewrite wordToNat_natToWord_idempotent in l0.
-    omega.
-    apply Nomega.Nlt_in; rewrite Nnat.Nat2N.id, Npow2_nat; assumption.
-    elimtype False.
-    apply n0.
-    rewrite <- (natToWord_wordToNat w).
-    rewrite !natToWord_plus.
-    rewrite !wordToNat_natToWord_idempotent.
-    rewrite <- natToWord_plus.
-    rewrite !wordToNat_natToWord_idempotent.
-    omega.
-    apply Nomega.Nlt_in; rewrite Nnat.Nat2N.id, Npow2_nat; assumption.
-    apply Nomega.Nlt_in; rewrite Nnat.Nat2N.id, Npow2_nat; omega.
-    omega.
-  Qed.
-
-  Ltac collapse_word :=
-      match goal with
-      | |- DecodeBindOpt2
-             (decode_word (sz := ?sz) ?b ?cd)
-             (fun w b' cd' =>
-                DecodeBindOpt2 (decode_word (sz := ?sz') b' cd')
-                               (fun w' b' cd' => @?k w w' b' cd')) = _ =>
-        etransitivity;
-        [let H := fresh in
-         pose proof (@CollapseWord _ _ _ _ _ addD_addD_plus _ sz sz' b cd k);
-         apply H | ]
-      end.
-  rewrite If_Opt_Then_Else_DecodeBindOpt_swap.
+  rewrite (If_Opt_Then_Else_DecodeBindOpt_swap (cache := dns_list_cache)).
   unfold H; higher_order_reflexivity.
-  collapse_word.
-  collapse_word.
-  collapse_word.
-  collapse_word.
+  collapse_word addD_addD_plus.
+  collapse_word addD_addD_plus.
+  collapse_word addD_addD_plus.
+  collapse_word addD_addD_plus.
   first [ apply DecodeBindOpt2_under_bind; simpl; intros
         | eapply optimize_under_if_bool; simpl; intros
         | eapply optimize_under_if; simpl; intros].
-  collapse_word.
-  collapse_word.
+  collapse_word addD_addD_plus.
+  collapse_word addD_addD_plus.
   higher_order_reflexivity.
   Defined.
 
-  Definition packetDecoderImpl := Eval simpl in (projT1 packet_decoder).
+  Definition packetDecoderImpl
+    := Eval simpl in (projT1 packet_decoder).
+
+  Lemma AlignedDecodeChar {C}
+        {numBytes}
+    : forall (v : Vector.t (word 8) (S numBytes))
+             (k : (word 8) -> ByteString -> CacheDecode -> option (C * ByteString * CacheDecode))
+             cd,
+    (`(a, b0, d) <- decode_word
+      (transformerUnit := ByteString_QueueTransformerOpt) (sz := 8) (build_aligned_ByteString v) cd;
+       k a b0 d) =
+    Let n := (Vector.nth v Fin.F1) in
+        k n (build_aligned_ByteString (Vector.tl v)) (addD cd 8).
+Proof.
+  unfold LetIn; intros.
+  unfold decode_word, WordOpt.decode_word.
+  rewrite aligned_decode_char_eq; simpl.
+  f_equal.
+  pattern numBytes, v; apply Vector.caseS; simpl; intros.
+  reflexivity.
+Qed.
+
+Lemma AlignedDecode2Char {C}
+        {numBytes}
+    : forall (v : Vector.t (word 8) (S (S numBytes)))
+             (k : (word 16) -> ByteString -> CacheDecode -> option (C * ByteString * CacheDecode))
+             cd,
+    (`(a, b0, d) <- decode_word
+      (transformerUnit := ByteString_QueueTransformerOpt) (sz := 16) (build_aligned_ByteString v) cd;
+       k a b0 d) =
+    Let n := Core.append_word (Vector.nth v (Fin.FS Fin.F1)) (Vector.nth v Fin.F1) in
+        k n (build_aligned_ByteString (Vector.tl (Vector.tl v))) (addD cd 16).
+Proof.
+  unfold LetIn; intros.
+  unfold decode_word, WordOpt.decode_word.
+  match goal with
+    |- context[Ifopt ?Z as _ Then _ Else _] => replace Z with
+                                               (let (v', v'') := Vector_split 2 numBytes v in Some (VectorByteToWord v', build_aligned_ByteString v'')) by (symmetry; apply (@aligned_decode_char_eq' _ 1 v))
+  end.
+  unfold Vector_split, If_Opt_Then_Else, DecodeBindOpt2 at 1, If_Opt_Then_Else.
+  f_equal.
+  rewrite !Vector_nth_tl, !Vector_nth_hd.
+  erewrite VectorByteToWord_cons.
+  rewrite <- !Eqdep_dec.eq_rect_eq_dec; eauto using Peano_dec.eq_nat_dec.
+  f_equal.
+  erewrite VectorByteToWord_cons.
+  rewrite <- !Eqdep_dec.eq_rect_eq_dec; eauto using Peano_dec.eq_nat_dec.
+  Grab Existential Variables.
+  omega.
+  omega.
+Qed.
+
+Corollary AlignedDecode2Nat {C}
+        {numBytes}
+    : forall (v : Vector.t (word 8) (S (S numBytes)))
+             (k : nat -> ByteString -> CacheDecode -> option (C * ByteString * CacheDecode))
+             cd,
+    (`(a, b0, d) <- decode_nat
+      (transformerUnit := ByteString_QueueTransformerOpt) 16 (build_aligned_ByteString v) cd;
+       k a b0 d) =
+    Let n := wordToNat (Core.append_word (Vector.nth v (Fin.FS Fin.F1)) (Vector.nth v Fin.F1)) in
+        k n (build_aligned_ByteString (Vector.tl (Vector.tl v))) (addD cd 16).
+Proof.
+  unfold decode_nat; intros.
+  rewrite DecodeBindOpt2_assoc.
+  unfold DecodeBindOpt2 at 2, If_Opt_Then_Else.
+  rewrite AlignedDecode2Char.
+  reflexivity.
+Qed.
+
+Lemma optimize_under_if_opt {A ResultT}
+  : forall (a_opt : option A) (t t' : A -> ResultT) (e e' : ResultT),
+    (forall a, t a = t' a) -> e = e' ->
+    Ifopt a_opt as a Then t a Else e = Ifopt a_opt as a Then t' a Else e'.
+Proof.
+  intros; subst; eauto.
+  destruct a_opt; eauto.
+Qed.
+
+Lemma rewrite_under_LetIn
+      {A B}
+  : forall (a : A) (k k' : A -> B),
+    (forall a, k a = k' a) -> LetIn a k = LetIn a k'.
+Proof.
+  intros; unfold LetIn; eauto.
+Qed.
+
+Fixpoint Guarded_Vector_split
+         (sz n : nat)
+         {struct sz}
+  : Vector.t (word 8) n
+    -> Vector.t (word 8) (sz + (n - sz)) :=
+  match sz, n return
+        Vector.t _ n
+        -> Vector.t (word 8) (sz + (n - sz))
+  with
+  | 0, _ => fun v => (eq_rect _ (Vector.t _) v _ (minus_n_O n))
+  | S n', 0 =>
+    fun v =>
+      Vector.cons _ (wzero _) _ (Guarded_Vector_split n' _ v)
+  | S n', S sz' =>
+    fun v =>
+      Vector.cons _ (Vector.hd v) _ (Guarded_Vector_split n' _ (Vector.tl v))
+  end .
+
+Lemma le_B_Guarded_Vector_split
+      {n}
+      (b : Vector.t _ n)
+      (m : nat)
+  : {b' : ByteString | le_B b' (build_aligned_ByteString b)}.
+  eexists (build_aligned_ByteString
+             (snd (Vector_split _ _ (Guarded_Vector_split m n b)))).
+  abstract (unfold build_aligned_ByteString, le_B; simpl; omega).
+Defined.
+
+Lemma Decode_w_Measure_le_eq'':
+  forall (A B : Type) (cache : Cache) (transformer : Transformer B)
+         (A_decode : B -> CacheDecode -> option (A * B * CacheDecode))
+         (b : B) (cd : CacheDecode)
+         (A_decode_le : forall (b0 : B) (cd0 : CacheDecode) (a : A) (b' : B) (cd' : CacheDecode),
+             A_decode b0 cd0 = Some (a, b', cd') -> le_B b' b0),
+    Decode_w_Measure_le A_decode b cd A_decode_le = None ->
+    A_decode b cd = None.
+Proof.
+  clear; intros ? ? ? ? ? ? ? ?; unfold Decode_w_Measure_le in *.
+  remember (A_decode_le b cd); clear Heql.
+  destruct (A_decode b cd) as [ [ [? ?] ? ] | ]; eauto.
+  intros; discriminate.
+Qed.
+
+Lemma build_aligned_ByteString_eq_split
+  : forall m n b H0,
+    (m <= n)%nat
+    -> build_aligned_ByteString b =
+       (build_aligned_ByteString (eq_rect (m + (n - m)) (t (word 8)) (Guarded_Vector_split m n b) n H0)).
+Proof.
+  intros.
+  intros; eapply ByteString_f_equal; simpl.
+  instantiate (1 := eq_refl _); reflexivity.
+  instantiate (1 := eq_refl _).
+  simpl.
+  revert n b H0 H; induction m; simpl.
+  intros ? ?; generalize (minus_n_O n).
+  intros; rewrite <- Equality.transport_pp.
+  apply Eqdep_dec.eq_rect_eq_dec; auto with arith.
+  intros.
+  inversion H; subst.
+  - revert b H0 IHm; clear.
+    intro; pattern m, b; apply Vector.caseS; simpl; intros.
+    assert ((n + (n - n)) = n) by omega.
+    rewrite eq_rect_Vector_cons with (H' := H).
+    f_equal.
+    erewrite <- IHm; eauto.
+  - revert b H0 IHm H1; clear.
+    intro; pattern m0, b; apply Vector.caseS; simpl; intros.
+    assert ((m + (n - m)) = n) by omega.
+    erewrite eq_rect_Vector_cons with (H' := H).
+    f_equal.
+    erewrite <- IHm; eauto.
+    omega.
+Qed.
+
+Lemma ByteAlign_Decode_w_Measure_le {A}
+  : forall (dec_a : ByteString -> CacheDecode -> option (A * ByteString * CacheDecode))
+           (n m : nat)
+           (dec_a' : Vector.t (word 8) (m + (n - m)) -> A)
+           (cd : CacheDecode)
+           (f : CacheDecode -> CacheDecode)
+           (b : Vector.t (word 8) n)
+           decode_a_le
+           (dec_fail : ~ (m <= n)%nat
+                       -> forall b cd, dec_a (build_aligned_ByteString (numBytes := n) b) cd = None),
+    (forall b cd, dec_a (build_aligned_ByteString b) cd =
+                  Some (dec_a' b, build_aligned_ByteString (snd (Vector_split m (n - m) b)), f cd))
+    -> Decode_w_Measure_le dec_a (build_aligned_ByteString b) cd decode_a_le =
+       If NPeano.leb m n Then
+          Let a := dec_a' (Guarded_Vector_split m n b) in
+      Some (a, le_B_Guarded_Vector_split b m, f cd)
+           Else None.
+Proof.
+  intros.
+  destruct (NPeano.leb m n) eqn: ?.
+  apply NPeano.leb_le in Heqb0.
+  simpl.
+  assert (m + (n - m) = n) by omega.
+  assert (forall b, Decode_w_Measure_le dec_a (build_aligned_ByteString b) cd decode_a_le
+                    = Decode_w_Measure_le dec_a (build_aligned_ByteString ( eq_rect _ _ (Guarded_Vector_split m n b) _ H0)) cd decode_a_le).
+  { revert Heqb0; clear; intros.
+    destruct (Decode_w_Measure_le dec_a (build_aligned_ByteString b) cd decode_a_le)
+      as [ [ [? [? ?] ] ?] | ] eqn: ?.
+    apply Decode_w_Measure_le_eq' in Heqo.
+    simpl in Heqo.
+    destruct (Decode_w_Measure_le dec_a
+                                  (build_aligned_ByteString (eq_rect (m + (n - m)) (t (word 8)) (Guarded_Vector_split m n b) n H0)) cd decode_a_le) as [ [ [? [? ?] ] ?] | ] eqn: ?.
+    apply Decode_w_Measure_le_eq' in Heqo0.
+    simpl in *.
+    rewrite <- build_aligned_ByteString_eq_split in Heqo0 by eauto.
+    rewrite Heqo0 in Heqo.
+    injection Heqo; intros.
+    rewrite H, H2;
+      repeat f_equal.
+    revert l l0. rewrite H1; intros; f_equal.
+    f_equal; apply Core.le_uniqueness_proof.
+    apply ByteString_id.
+    eapply Decode_w_Measure_le_eq'' in Heqo0.
+    rewrite <- build_aligned_ByteString_eq_split in Heqo0 by eauto.
+    rewrite Heqo0 in Heqo.
+    discriminate.
+    apply ByteString_id.
+    erewrite build_aligned_ByteString_eq_split in Heqo by eauto.
+    rewrite Heqo; reflexivity.
+  }
+  rewrite H1.
+  match goal with
+    |- ?a = _ => destruct a as [ [ [? ?] ? ] | ] eqn: ?
+  end.
+  eapply Decode_w_Measure_le_eq' in Heqo.
+  assert (dec_a (build_aligned_ByteString (Guarded_Vector_split m n b)) cd
+          = Some (a, projT1 s, c)).
+  { destruct s; simpl in *.
+    rewrite <- Heqo.
+    unfold build_aligned_ByteString; repeat f_equal; simpl.
+    eapply ByteString_f_equal; simpl.
+    instantiate (1 := eq_refl _); reflexivity.
+    instantiate (1 := sym_eq H0).
+    clear H1.
+    destruct H0; reflexivity.
+  }
+  rewrite H in H2; injection H2; intros.
+  rewrite H3, H5; unfold LetIn; simpl.
+  repeat f_equal.
+  destruct s; simpl in *.
+  unfold le_B_Guarded_Vector_split; simpl.
+  clear H1; revert l.
+  rewrite <- H4; intros.
+  f_equal; apply Core.le_uniqueness_proof.
+  apply ByteString_id.
+  apply Decode_w_Measure_le_eq'' in Heqo.
+  pose proof (H (Guarded_Vector_split m n b) cd).
+  assert (Some (dec_a' (Guarded_Vector_split m n b),
+                build_aligned_ByteString (snd (Vector_split m (n - m) (Guarded_Vector_split m n b))),
+                f cd) = None).
+  { rewrite <- Heqo.
+    rewrite <- H.
+    repeat f_equal.
+    eapply ByteString_f_equal; simpl.
+    instantiate (1 := eq_refl _); reflexivity.
+    instantiate (1 := sym_eq H0).
+    clear H1.
+    destruct H0; reflexivity.
+  }
+  discriminate.
+  assert (~ m <= n)%nat by (rewrite <- NPeano.leb_le; congruence).
+  eapply dec_fail in H0; simpl.
+  eapply Specs.Decode_w_Measure_le_eq' in H0.
+  apply H0.
+Qed.
+
+Lemma lt_B_Guarded_Vector_split
+      {n}
+      (b : Vector.t _ n)
+      (m : nat)
+      (_ : lt m n)
+  : {b' : ByteString | lt_B b' (build_aligned_ByteString b)}.
+  eexists (build_aligned_ByteString
+             (snd (Vector_split _ _ (Guarded_Vector_split (S m) n b)))).
+  abstract (unfold build_aligned_ByteString, lt_B; simpl; omega).
+Defined.
+
+Lemma Decode_w_Measure_lt_eq'':
+  forall (A B : Type) (cache : Cache) (transformer : Transformer B)
+         (A_decode : B -> CacheDecode -> option (A * B * CacheDecode))
+         (b : B) (cd : CacheDecode)
+         (A_decode_lt : forall (b0 : B) (cd0 : CacheDecode) (a : A) (b' : B) (cd' : CacheDecode),
+             A_decode b0 cd0 = Some (a, b', cd') -> lt_B b' b0),
+    Decode_w_Measure_lt A_decode b cd A_decode_lt = None ->
+    A_decode b cd = None.
+Proof.
+  clear; intros ? ? ? ? ? ? ? ?; unfold Decode_w_Measure_lt in *.
+  remember (A_decode_lt b cd); clear Heql.
+  destruct (A_decode b cd) as [ [ [? ?] ? ] | ]; eauto.
+  discriminate.
+Qed.
+
+Arguments Guarded_Vector_split : simpl never.
+
+Lemma ByteAlign_Decode_w_Measure_lt {A}
+  : forall (dec_a : ByteString -> CacheDecode -> option (A * ByteString * CacheDecode))
+           (n m : nat)
+           (dec_a' : Vector.t (word 8) (S m + (n - (S m))) -> A)
+           (cd : CacheDecode)
+           (f : CacheDecode -> CacheDecode)
+           (b : Vector.t (word 8) n)
+           decode_a_le
+           (dec_fail : ~ (lt m n)%nat
+                       -> forall b cd, dec_a (build_aligned_ByteString (numBytes := n) b) cd = None),
+    (forall b cd, dec_a (build_aligned_ByteString b) cd =
+                  Some (dec_a' b, build_aligned_ByteString (snd (Vector_split (S m) (n - (S m)) b)), f cd))
+    -> Decode_w_Measure_lt dec_a (build_aligned_ByteString b) cd decode_a_le =
+       match Compare_dec.lt_dec m n with
+       | left e =>
+         (Let a := dec_a' (Guarded_Vector_split (S m) n b) in
+              Some (a, lt_B_Guarded_Vector_split b m e, f cd))
+       | right _ => None
+       end.
+Proof.
+  intros.
+  destruct (Compare_dec.lt_dec m n).
+  simpl.
+  assert (S m + (n - (S m)) = n) by omega.
+  assert (forall b, Decode_w_Measure_lt dec_a (build_aligned_ByteString b) cd decode_a_le
+                    = Decode_w_Measure_lt dec_a (build_aligned_ByteString ( eq_rect _ _ (Guarded_Vector_split (S m) n b) _ H0)) cd decode_a_le).
+  { revert l; clear; intros.
+    destruct (Decode_w_Measure_lt dec_a (build_aligned_ByteString b) cd decode_a_le)
+      as [ [ [? [? ?] ] ?] | ] eqn: ?.
+    apply Decode_w_Measure_lt_eq' in Heqo.
+    simpl in Heqo.
+    destruct (Decode_w_Measure_lt dec_a
+                                  (build_aligned_ByteString (eq_rect _ (t (word 8)) (Guarded_Vector_split (S m) n b) n H0)) cd decode_a_le) as [ [ [? [? ?] ] ?] | ] eqn: ?.
+    apply Decode_w_Measure_lt_eq' in Heqo0.
+    unfold proj1_sig in Heqo0.
+    rewrite <- build_aligned_ByteString_eq_split in Heqo0.
+    rewrite Heqo0 in Heqo.
+    injection Heqo; intros.
+    rewrite H, H2;
+      repeat f_equal.
+    revert l1 l0. rewrite H1; intros; f_equal.
+    f_equal; apply Core.le_uniqueness_proof.
+    omega.
+    apply ByteString_id.
+    eapply Decode_w_Measure_lt_eq'' in Heqo0.
+    rewrite <- build_aligned_ByteString_eq_split in Heqo0 by omega.
+    rewrite Heqo0 in Heqo.
+    discriminate.
+    apply ByteString_id.
+    erewrite build_aligned_ByteString_eq_split in Heqo by eauto.
+    rewrite Heqo; reflexivity.
+  }
+  rewrite H1.
+  match goal with
+    |- ?a = _ => destruct a as [ [ [? ?] ? ] | ] eqn: ?
+  end.
+  eapply Decode_w_Measure_lt_eq' in Heqo.
+  assert (dec_a (build_aligned_ByteString (Guarded_Vector_split (S m) n b)) cd
+          = Some (a, projT1 s, c)).
+  { destruct s; simpl in *.
+    rewrite <- Heqo.
+    unfold build_aligned_ByteString; repeat f_equal; simpl.
+    eapply ByteString_f_equal; simpl.
+    instantiate (1 := eq_refl _); reflexivity.
+    instantiate (1 := sym_eq H0).
+    clear H1.
+    destruct H0; reflexivity.
+  }
+  rewrite H in H2; injection H2; intros.
+  rewrite H3, H5; unfold LetIn; simpl.
+  repeat f_equal.
+  destruct s; simpl in *.
+  unfold lt_B_Guarded_Vector_split; simpl.
+  clear H1; revert l0.
+  rewrite <- H4; intros.
+  f_equal; apply Core.le_uniqueness_proof.
+  apply ByteString_id.
+  apply Decode_w_Measure_lt_eq'' in Heqo.
+  pose proof (H (Guarded_Vector_split (S m) n b) cd).
+  assert (Some (dec_a' (Guarded_Vector_split (S m) n b),
+                build_aligned_ByteString (snd (Vector_split (S m) (n - (S m)) (Guarded_Vector_split (S m) n b))),
+                f cd) = None).
+  { rewrite <- Heqo.
+    rewrite <- H.
+    repeat f_equal.
+    eapply ByteString_f_equal; simpl.
+    instantiate (1 := eq_refl _); reflexivity.
+    instantiate (1 := sym_eq H0).
+    clear H1.
+    destruct H0; reflexivity.
+  }
+  discriminate.
+  eapply dec_fail in n0; simpl.
+  eapply Specs.Decode_w_Measure_lt_eq' in n0.
+  apply n0.
+Qed.
+
+Print decode_DomainName.
+
+Lemma optimize_Fix {A}
+  : forall
+    (body : forall x : ByteString,
+        (forall y : ByteString,
+            lt_B y x -> (fun _ : ByteString => CacheDecode -> option (A * ByteString * CacheDecode)) y) ->
+        (fun _ : ByteString => CacheDecode -> option (A * ByteString * CacheDecode)) x)
+    (body' : forall x : nat,
+        (forall y : nat,
+            (lt y x)%nat ->
+            (fun m : nat =>
+               t (word 8) m -> CacheDecode ->
+               option (A * {n : _ & Vector.t _ n} * CacheDecode)) y) ->
+        t (word 8) x -> CacheDecode -> option (A * {n : _ & Vector.t _ n} * CacheDecode) )
+    n (b : Vector.t _ n) (cd : CacheDecode)
+    (body_Proper :
+       forall (x0 : ByteString)
+              (f g : forall y : ByteString, lt_B y x0 -> CacheDecode -> option (A * ByteString * CacheDecode)),
+         (forall (y : ByteString) (p : lt_B y x0), f y p = g y p) -> body x0 f = body x0 g)
+    (body'_Proper :
+       forall (x0 : nat)
+              (f
+                 g : forall y : nat,
+                  (lt y x0)%nat -> t (word 8) y -> CacheDecode -> option (A * {n0 : nat & t Core.char n0} * CacheDecode)),
+         (forall (y : nat) (p : (lt y x0)%nat), f y p = g y p) -> body' x0 f = body' x0 g)
+  ,
+    (forall n (b : Vector.t (word 8) n)
+            (rec : forall x : ByteString,
+                lt_B x (build_aligned_ByteString b) -> CacheDecode -> option (A * ByteString * CacheDecode))
+            (rec' : forall x : nat,
+                (lt x n)%nat -> t Core.char x -> CacheDecode ->
+                option (A * {n : _ & Vector.t _ n} * CacheDecode))
+            cd,
+        (forall m cd b a b' cd' b_lt b_lt' ,
+            rec' m b_lt' b cd = Some (a, b', cd')
+            -> rec (build_aligned_ByteString b) b_lt cd = Some (a, build_aligned_ByteString (projT2 b'), cd'))
+        -> body (build_aligned_ByteString b) rec cd
+           = match (body' n rec' b cd) with
+             | Some (a, b', cd') => Some (a, build_aligned_ByteString (projT2 b'), cd')
+             | None => None
+             end)
+    -> Fix well_founded_lt_b (fun _ : ByteString => CacheDecode -> option (A * ByteString * CacheDecode)) body (build_aligned_ByteString b) cd =
+       match Fix Wf_nat.lt_wf (fun m : nat => Vector.t (word 8) m -> CacheDecode -> option (A * { n : _ & Vector.t _ n} * CacheDecode)) body' n b cd with
+       | Some (a, b', cd') => Some (a, build_aligned_ByteString (projT2 b'), cd')
+       | None => None
+       end.
+Proof.
+  intros.
+  revert cd b; pattern n.
+  eapply (well_founded_ind Wf_nat.lt_wf); intros.
+  rewrite Init.Wf.Fix_eq, Init.Wf.Fix_eq.
+  apply H; intros.
+  erewrite H0.
+  rewrite H1.
+  reflexivity.
+  omega.
+  eauto.
+  eauto.
+Qed.
+
+Definition ByteAligned_packetDecoderImpl n
+  : {impl : _ & forall (v : Vector.t _ (12 + n)),
+         fst packetDecoderImpl (build_aligned_ByteString v) (Some (wzero 17), @nil (pointerT * string)) =
+         impl v (Some (wzero 17) , @nil (pointerT * string))%list}.
+Proof.
+  eexists _; intros.
+  etransitivity.
+  set_refine_evar; simpl.
+  rewrite (@AlignedDecode2Char _ ).
+  subst_refine_evar; apply rewrite_under_LetIn; intros; set_refine_evar.
+  rewrite (@AlignedDecodeChar _ ).
+  rewrite <- !Vector_nth_tl.
+  subst_refine_evar; apply rewrite_under_LetIn; intros; set_refine_evar.
+  rewrite (@AlignedDecodeChar _ ).
+  rewrite <- !Vector_nth_tl.
+  subst_refine_evar; apply rewrite_under_LetIn; intros; set_refine_evar.
+  subst_refine_evar.
+  etransitivity;
+    [eapply (If_Opt_Then_Else_DecodeBindOpt (cache := dns_list_cache))
+    | ].
+  eapply optimize_under_if_opt; simpl; intros.
+  etransitivity;
+    [eapply (If_Opt_Then_Else_DecodeBindOpt (cache := dns_list_cache))
+    | ].
+  eapply optimize_under_if_opt; simpl; intros.
+  eapply optimize_under_if; simpl; intros.
+  rewrite (@AlignedDecode2Nat _).
+  rewrite <- !Vector_nth_tl.
+  subst_refine_evar; apply rewrite_under_LetIn; intros; set_refine_evar.
+  eapply optimize_under_if; simpl; intros.
+  rewrite (@AlignedDecode2Nat _).
+  rewrite <- !Vector_nth_tl.
+  subst_refine_evar; apply rewrite_under_LetIn; intros; set_refine_evar.
+  rewrite (@AlignedDecode2Nat _).
+  rewrite <- !Vector_nth_tl.
+  subst_refine_evar; apply rewrite_under_LetIn; intros; set_refine_evar.
+  rewrite (@AlignedDecode2Nat _).
+  rewrite <- !Vector_nth_tl.
+  subst_refine_evar; apply rewrite_under_LetIn; intros; set_refine_evar.
+  rewrite DecodeBindOpt2_assoc.
+  unfold decode_DomainName.
+  2: reflexivity.
+  2: reflexivity.
+  2: reflexivity.
+  2: reflexivity.
+  erewrite optimize_Fix.
+  Focus 4.
+  etransitivity.
+  simpl; intros.
+  erewrite ByteAlign_Decode_w_Measure_le with (m := 1)
+                                                (dec_a' := Vector.hd)
+                                                (f := fun cd => addD cd 8);
+    try (intros; unfold decode_word; rewrite aligned_decode_char_eq;
+         reflexivity).
+  Focus 2.
+  intros; assert (n0 = 0) by omega; subst.
+  revert b0; clear.
+  apply case0; reflexivity.
+  set_refine_evar.
+  Lemma optimize_If_bind2_bool {A A' B B' C}
+    : forall (c : bool)
+             (t e : option (A * B * C))
+             (k : A -> B -> C -> option (A' * B' * C)),
+      (`(a, b, env) <- (If c Then t Else e); k a b env) =
+      If c Then `(a, b, env) <- t; k a b env Else (`(a, b, env) <- e; k a b env).
+  Proof.
+    destruct c; simpl; intros; reflexivity.
+  Qed.
+
+  rewrite optimize_If_bind2_bool.
+  subst H2.
+  eapply optimize_under_if_bool.
+  Lemma optimize_under_match {A B}
+    : forall (a a' : A) (f : {a = a'} + {a <> a'}) (t t' : _ -> B)
+             (e e' : _ -> B),
+      (forall (a a' : A) (a_eq : _), t a_eq = t' a_eq)
+      -> (forall (a a' : A) (a_neq : _), e a_neq = e' a_neq)
+      -> match f with
+          | left e => t e
+          | right n => e n
+         end =
+         match f with
+         | left e => t' e
+         | right n => e' n
+         end.
+  Proof.
+    destruct f; simpl; intros; eauto.
+  Qed.
+
+  apply optimize_under_match; intros.
+  simpl.
+  erewrite ByteAlign_Decode_w_Measure_le with (m := 1)
+                                                (dec_a' := Vector.hd)
+                                                (f := fun cd => addD cd 8);
+    try (intros; unfold decode_word; rewrite aligned_decode_char_eq;
+         reflexivity).
+  Focus 2.
+  intros; assert (n0 - 1 = 0) by omega.
+  revert b0; rewrite H3; clear.
+  apply case0; reflexivity.
+  set_refine_evar.
+  simpl.
+  rewrite optimize_If_bind2_bool.
+  eapply optimize_under_if_bool.
+  simpl.
+  reflexivity.
+  simpl.
+  reflexivity.
+  eapply optimize_under_if_bool.
+  apply optimize_under_match.
+  simpl.
+  intros; higher_order_reflexivity.
+  intros.
+  simpl.
+  2: reflexivity.
+  2: reflexivity.
+  2: simpl.
+  erewrite ByteAlign_Decode_w_Measure_lt with (m := (wordToNat (Vector.hd (Guarded_Vector_split 1 n0 b)))).
+  Focus 3.
+  match goal with
+    |- (DecodeBindOpt2 (If_Then_Else ?i ?t ?e) ?k) = _ =>
+    pose proof (fun A B C C' => @optimize_if_bind2_bool A B C C' i);
+      pose i; pose t; pose e; pose k
+  end.
+  Check (H3 _ _ _ _ o o0 o1).
+
+
+  clear H.
+
+  idtac.
+
+  Focus 2.
+  unfold Decode_w_Measure_le.
+  destruct (dec_a (build_aligned_ByteString b) cd).
 
   Print packetDecoderImpl.
 
